polishing

LeanLangur/Draft/StackMachine.lean
@@ -7,6 +7,8 @@ inductive Instr
   | add
   deriving Repr
 
+open Instr
+
 abbrev Stack := List Nat
 
 abbrev Program := List Instr
@@ -14,10 +16,10 @@ abbrev Program := List Instr
 def eval! (p: Program) (s: Stack) : Stack :=
   match p with
   | [] => s
-  | Instr.push n :: p' => eval! p' (n :: s)
-  | Instr.pop :: p' =>
+  | push n :: p' => eval! p' (n :: s)
+  | pop :: p' =>
       eval! p' s.tail!
-  | Instr.add :: p' =>
+  | add :: p' =>
       let x := s.head!
       let y := s.tail!.head!
       eval! p' ((x + y) :: s.tail!.tail!)
@@ -25,12 +27,12 @@ def eval! (p: Program) (s: Stack) : Stack :=
 def eval? (p: Program) (s: Stack) : Option Stack :=
   match p with
   | [] => some s
-  | Instr.push n :: p' => eval? p' (n :: s)
-  | Instr.add :: p' =>
+  | push n :: p' => eval? p' (n :: s)
+  | add :: p' =>
       match s with
       | x :: y :: zs => eval? p' ((x + y) :: zs)
       | _ => none
-  | Instr.pop :: p' =>
+  | pop :: p' =>
       match s with
       | _ :: ys => eval? p' ys
       | _ => none
@@ -40,105 +42,153 @@ def eval? (p: Program) (s: Stack) : Option Stack :=
 inductive ValidProgram : (initStackSize : Nat) → (p : Program) → Prop
   /-- The empty program is valid with any initial stack -/
   | nil : ValidProgram n []
-  /-- If the first instruction is a push and the rest of the program is valid  with stack size `s + 1` then the program is valid with initial stack size `s` -/
+  /-- If the first instruction is a push and the rest of the program is valid  with initial stack size `s + 1` then the program is valid with initial stack size `s` -/
   | push  {p : Program} :
       ValidProgram (n + 1) p →
-      ValidProgram n (Instr.push k :: p)
-  /-- If the first instruction is a pop and the rest of the program is valid with stack size `s` then the program is valid with initial stack size `s + 1` -/
+      ValidProgram n (push k :: p)
+  /-- If the first instruction is a pop and the rest of the program is valid with initial stack size `s` then the program is valid with initial stack size `s + 1` -/
   | pop  {p : Program} :
       ValidProgram n p →
-      ValidProgram (n + 1) (Instr.pop :: p)
-  /-- If the first instruction is an add and the rest of the program is valid with stack size `s + 2` then the program is valid with initial stack size `s + 1` -/
+      ValidProgram (n + 1) (pop :: p)
+  /-- If the first instruction is an add and the rest of the program is valid with initial stack size `s + 2` then the program is valid with initial stack size `s + 1` -/
   | add {p : Program} :
       ValidProgram (n + 1) p →
-      ValidProgram (n + 2) (Instr.add :: p)
+      ValidProgram (n + 2) (add :: p)
 
 @[simp, grind .]
 theorem valid_program_nil : ValidProgram n [] := ValidProgram.nil
 
 @[simp, grind .]
 theorem valid_program_push (n: Nat) (h : ValidProgram (n + 1) p') :
-    ValidProgram n (Instr.push k :: p') :=    ValidProgram.push h
+    ValidProgram n (push k :: p') :=    ValidProgram.push h
 
 @[simp, grind .]
 theorem valid_program_add (k: Nat) (h : ValidProgram (k + 1) p') :
-  ValidProgram (k + 2) (Instr.add :: p') :=
+  ValidProgram (k + 2) (add :: p') :=
   ValidProgram.add h
 
 @[simp]
 theorem valid_program_pop (h : ValidProgram n p') :
-  ValidProgram (n + 1) (Instr.pop :: p') :=
+  ValidProgram (n + 1) (pop :: p') :=
   ValidProgram.pop h
 
-example (a b: Nat) : ValidProgram 0 [Instr.push a, Instr.push b, Instr.add] := by
+example (a b: Nat) : ValidProgram 0 [push a, push b, add] := by
   grind
 
-example (a b c : Nat) : ValidProgram 0 [Instr.push a, Instr.push b, Instr.add, Instr.push c, Instr.add] := by
+example (a b c : Nat) : ValidProgram 0 [push a, push b, add, push c, add] := by
   grind (ematch := 7)
 
 @[simp]
-theorem valid_program_of_push {k: Nat} (h : ValidProgram k (Instr.push a :: p')) : ValidProgram (k + 1) p' := by
+theorem valid_program_of_push {k: Nat} (h : ValidProgram k (push a :: p')) : ValidProgram (k + 1) p' := by
   cases h
   assumption
 
 
 @[simp]
-theorem invalid_program_add_zero: ¬ ValidProgram 0 (Instr.add :: p')  := by
+theorem invalid_program_add_zero: ¬ ValidProgram 0 (add :: p')  := by
   intro h
   cases h
 
 @[simp]
-theorem invalid_program_add_one: ¬ ValidProgram 1 (Instr.add :: p')  := by
+theorem invalid_program_add_one: ¬ ValidProgram 1 (add :: p')  := by
   grind
   -- intro h
   -- cases h
 
 @[simp]
-theorem valid_program_of_add {k: Nat} (h : ValidProgram (k + 2) (Instr.add :: p')) : ValidProgram (k + 1) p' := by
+theorem valid_program_of_add {k: Nat} (h : ValidProgram (k + 2) (add :: p')) : ValidProgram (k + 1) p' := by
   grind
 
 @[simp]
-theorem invalid_program_pop_zero: ¬ ValidProgram 0 (Instr.pop :: p')  := by
+theorem invalid_program_pop_zero: ¬ ValidProgram 0 (pop :: p')  := by
   grind
 
 @[simp]
-theorem valid_program_of_pop {k: Nat} (h : ValidProgram (k +1) (Instr.pop :: p')) : ValidProgram k p' := by
+theorem valid_program_of_pop {k: Nat} (h : ValidProgram (k +1) (pop :: p')) : ValidProgram k p' := by
   grind
 
 def evaluate (p: Program) (initStack: Stack) (h: ValidProgram initStack.length p) : Stack :=
   match p with
   | [] => initStack
-  | Instr.push n :: p' =>
+  | push n :: p' =>
       evaluate p' (n :: initStack) (valid_program_of_push h)
-  | Instr.add :: p' =>
+  | add :: p' =>
       match initStack with
       | x :: y :: zs =>
         evaluate p' ((x + y) :: zs) (valid_program_of_add h)
       | [x] => by
         simp at h
-  | Instr.pop :: p' =>
+  | pop :: p' =>
       match initStack with
       | [] => by
         simp at h
       | x :: ys => evaluate p' ys (valid_program_of_pop h)
 
+#eval evaluate [push 2, push 3, add] [] (by grind)
+
+#eval evaluate [push 2, add] [3] (by grind)
+
+/--
+error: `grind` failed
+case grind
+h : ¬ValidProgram [].length [push 2, add]
+⊢ False
+[grind] Goal diagnostics
+  [facts] Asserted facts
+    [prop] ¬ValidProgram [].length [push 2, add]
+    [prop] [].length = 0
+    [prop] ValidProgram ([].length + 1) [add] → ValidProgram [].length [push 2, add]
+  [eqc] True propositions
+    [prop] [].length = 0
+    [prop] ValidProgram ([].length + 1) [add] → ValidProgram [].length [push 2, add]
+  [eqc] False propositions
+    [prop] ValidProgram [].length [push 2, add]
+    [prop] ValidProgram ([].length + 1) [add]
+  [eqc] Equivalence classes
+    [eqc] {[].length, 0}
+    [eqc] others
+      [eqc] {↑[].length, ↑0}
+  [ematch] E-matching patterns
+    [thm] List.eq_nil_of_length_eq_zero: [@List.length #2 #1]
+    [thm] List.length_nil: [@List.length #0 (@List.nil _)]
+    [thm] List.length_cons: [@List.length #2 (@List.cons _ #1 #0)]
+    [thm] valid_program_nil: [ValidProgram #0 `[[]]]
+    [thm] valid_program_push: [ValidProgram #1 (@List.cons `[Instr] (push #2) #3)]
+    [thm] valid_program_add: [ValidProgram (#1 + 2) (@List.cons `[Instr] `[add] #2)]
+  [cutsat] Assignment satisfying linear constraints
+    [assign] [].length := 0
+  [ring] Rings
+    [ring] Ring `Lean.Grind.Ring.OfSemiring.Q Nat`
+      [basis] Basis
+        [_] ↑[].length = 0
+    [ring] Ring `Int`
+      [basis] Basis
+        [_] ↑[].length = 0
+[grind] Diagnostics
+  [thm] E-Matching instances
+    [thm] List.eq_nil_of_length_eq_zero ↦ 1
+    [thm] List.length_nil ↦ 1
+    [thm] valid_program_push ↦ 1
+-/
+#guard_msgs in
+#eval evaluate [push 2, add] [] (by grind)
 
 theorem valid_iff_eval?_some (p: Program) (s: Stack) : ValidProgram s.length p ↔ (eval? p s) ≠ none := by
   constructor
   · intro h
     match p with
     | [] => grind [eval?]
-    | Instr.push n :: p' =>
+    | push n :: p' =>
         have h' : ValidProgram (s.length + 1) p' := valid_program_of_push h
         have ih := (valid_iff_eval?_some p' (n ::s))
         grind [eval?]
-    | Instr.add :: p' =>
+    | add :: p' =>
         match s with
         | x :: y :: zs =>
            have h' := valid_program_of_add h
            have ih := (valid_iff_eval?_some p' ((x + y) :: zs))
            grind [eval?]
-    | Instr.pop :: p' =>
+    | pop :: p' =>
         match s with
         | x :: ys =>
             have h' : ValidProgram ys.length p' := valid_program_of_pop h
@@ -147,15 +197,15 @@ theorem valid_iff_eval?_some (p: Program) (s: Stack) : ValidProgram s.length p �
   · intro h
     match p with
     | [] => grind [eval?]
-    | Instr.push n :: p' =>
+    | push n :: p' =>
         have ih := (valid_iff_eval?_some p' (n ::s))
         grind [eval?]
-    | Instr.add :: p' =>
+    | add :: p' =>
         match s with
         | x :: y :: zs =>
            have ih := (valid_iff_eval?_some p' ((x + y) :: zs))
            grind [eval?]
-    | Instr.pop :: p' =>
+    | pop :: p' =>
         match s with
         | x :: ys =>
             have ih := (valid_iff_eval?_some p' ys)
