LeanLangur/Draft/Adders.lean
@@ -1,0 +1,15 @@
+namespace langur
+
+instance : HAdd α (List α) (List α) where
+  hAdd x xs := x :: xs
+
+#eval 3 + [4, 5]
+
+instance {α β : Type} [HAdd α α α][HAdd β β β] : HAdd (α × β) (α × β) (α × β) where
+  hAdd := fun (a, b) (c, d) ↦ (a + c, b + d)
+
+#eval (3, 4) + (5, 6)
+
+#eval (3, 4, 5) + (6, 7, 8)
+
+end langur
