LeanLangur/Draft/NonAtom.lean
@@ -1,0 +1,50 @@
+class NonAtom (α : Type) where
+    firstAtom : α
+    secondAtom : α
+    firstNeqSecond : firstAtom ≠ secondAtom
+
+def firstAtom (α : Type) [c: NonAtom α] : α := c.firstAtom
+def secondAtom (α : Type) [c: NonAtom α] : α := c.secondAtom
+theorem firstAtomNeqSecond (α : Type) [c: NonAtom α] : firstAtom α  ≠ secondAtom α := c.firstNeqSecond
+
+instance : NonAtom Nat where
+    firstAtom := 0
+    secondAtom := 1
+    firstNeqSecond := by decide
+
+instance: NonAtom Bool where
+    firstAtom := false
+    secondAtom := true
+    firstNeqSecond := by decide
+
+instance [NonAtom α] : NonAtom (List α) where
+    firstAtom := []
+    secondAtom := [firstAtom α]
+    firstNeqSecond := by simp
+
+instance [Inhabited α] : NonAtom (Option α) where
+    firstAtom := none
+    secondAtom := some (default : α)
+    firstNeqSecond := by simp
+
+instance [NonAtom α] : NonAtom (α × α) where
+    firstAtom := (firstAtom α, firstAtom α)
+    secondAtom := (secondAtom α, secondAtom α)
+    firstNeqSecond := by simp [firstAtomNeqSecond α]
+
+instance [NonAtom α] : Inhabited α where
+    default := firstAtom α
+
+instance [NonAtom α] [Inhabited β] : NonAtom (α × β) where
+    firstAtom := (firstAtom α, (default : β))
+    secondAtom := (secondAtom α, (default : β))
+    firstNeqSecond := by simp [firstAtomNeqSecond α]
+
+instance [Inhabited α] [NonAtom β] : NonAtom (α × β) where
+    firstAtom := ((default : α), firstAtom β)
+    secondAtom := ((default : α), secondAtom β)
+    firstNeqSecond := by simp [firstAtomNeqSecond β]
+
+#eval firstAtom <| Nat × Unit
+
+#eval secondAtom <| Nat × Nat
